Move version with dynamic alloc in old DepositSmart.dfy.

src/dafny/smart/DepositSmart.dfy
@@ -24,10 +24,14 @@ include "./trees/MerkleTrees.dfy"
 include "./algorithms/IndexBasedAlgorithm.dfy"
 
 /**
- *  A proof of correctness for the Deposit Smart Contract Algorithm.
+ *  A proof of correctness for the Deposit Smart Contract Algorithm
+ *  with dynamuc allocation of arrays.
+ *  This proof takes into account the allocations of arrays on the heap
+ *  and uses the Dafny dynamic frames support to reason about the
+ *  memory footprint (and to prove that no overwriting of array elements occur.)
  *  
  */
-module DepositSmart {
+module DepositSmartArrayAlloc {
 
     import opened ComputeRootPath
     import opened RSiblings
@@ -42,12 +46,17 @@ module DepositSmart {
 
     /**
      *  Provide deposit smart contract algorithms.
+     *
+     *  The autocontracts attribute generate some boilerplate 
+     *  code in the constructor and the methods. It also
+     *  implicitely adds to each method Valid() as a pre and
+     *  post-condition.
      */
     class {:autocontracts} Deposit {
 
         //  State Variables.
 
-        /** The default value for the leaves. It is 0 in the orginal algorithm. */
+        /** The default value for the leaves of the tree. It is 0 in the orginal algorithm. */
         const d : int 
 
         /** The attribute function to synthesise. Hash funciton in the original algorithm. */
@@ -56,20 +65,22 @@ module DepositSmart {
         /** The height of the tree. */
         const TREE_HEIGHT : nat
 
-        /** The values on the left siblings of the path to leaf at index k. */
-        ghost var rBranch : seq<int>
-
-        /** branch is rBranch in reverse order. */
+        /** branch is rBranch (see after) in reverse order. */
         var branch: array<int>
 
-        /** The values of the right siblings of the path to leaf at index k. */
-        ghost const zero_h : seq<int>
+        /** zero_hashes is zero_h (see below) in reverse order. */
         const zero_hashes: array<int> 
 
         /** The number of values added to the list. Also the index of the next available leaf. */
         var count : nat 
 
         //  Ghost variables used for the correctness proof.
+
+        /** The values on the left siblings of the path to leaf at index k. */
+        ghost var rBranch : seq<int>
+
+        /** The values of the right siblings of the path to leaf at index k. */
+        ghost const zero_h : seq<int>
 
         /** The list of values added so far. */
         ghost var values : seq<int> 
@@ -78,14 +89,12 @@ module DepositSmart {
 
         /** 
          *  @note   `values` record the values added so far. buildMerkle(values, TREE_HEIGHT, f, d)
-         *          is the Merkle tree that corresponds to `values`.
+         *          is the Merkle tree that corresponds to the list `values`.
          *          `rBranch` and `zero_h` should always contain the left (resp. right) siblings 
          *          of the path to the |values|-th leaf in the Merkle tree. 
-         *  @note   |values| is the length of the
-         *          list `values`.
+         *  @note   |values| is the length of the list `values`.
          */
         predicate Valid()
-            // reads this, this.zero_hashes, this.branch
         {
             //  Constraints on height and length of lists.
             1 <= TREE_HEIGHT == branch.Length == |rBranch| == |zero_h| 
@@ -114,111 +123,100 @@ module DepositSmart {
          *  @note           The initial value of `rBranch` is unconstrained (apart the length
          *                  that should be the same as `h`). This implies that the algorithms
          *                  are correct given any initial values for `rBranch`.
+         *  @note           The autocontracts attribute ensures that the post condition
+         *                   Valid() holds after the initilisation.
          */
         constructor(h: nat, l : seq<int>, f1 : (int, int) -> int, default : int) 
             requires h >= 1
             requires |l| == h 
-            // ensures fresh({zero_hashes} - {this})
-            ensures fresh({branch, zero_hashes})
-            // ensures fresh({branch} - {this.zero_hashes, this})
-            // ensures Valid()
-            // ensures branch == reverse(rBranch)
+            ensures branch != zero_hashes
         {
             //  State variables
             TREE_HEIGHT, count, f, d := h, 0, f1, default;
-            zero_h, rBranch := zeroes(f1, default, h - 1), reverse(l) ;
 
-            // zero_hashes := reverse(zeroes(f1, default, h - 1));
-            zero_hashes := new int[h](i requires 0 <= i < h  => zeroes(f1, default, h - 1)[h - 1 - i]);
-            // init_zero_hashes(zero_hashes, h, f1, default);
-            // zero_hashes[0] := default;
-            // var i := 0;
-            // while i < h {
-            //     i := i + 1;
-            // }
-
-            // zero_hashes := init_zero_hashes(h, f1, default);
-            // a := [];
-            //  Ghost variables
-           
-            values := [];
+            //  Allocate the array branch, and initialise with `l`.
             branch := new int[h](i requires 0 <= i < h => l[i]);
+
+            // Allocate the zeroes array.
+            zero_hashes := new int[h](i requires 0 <= i < h  => zeroes(f1, default, h - 1)[h - 1 - i]);
+    
+            //  Ghost variables
+            zero_h, rBranch := zeroes(f1, default, h - 1), reverse(l) ;
+            values := [];
+
             //  Proof that right siblings of path natToBitList2(0, h) are zero_h.
             bitToNatToBitsIsIdentity(0, h);
             valueIsZeroImpliesAllZeroes(natToBitList2(0, h));
             leafAtPathIsIntValueOfPath(natToBitList2(0, h), buildMerkle([], h, f1, default), 0, 0);
             rightSiblingsOfLastPathAreDefault(natToBitList2(0, h), buildMerkle([], h, f1, default), 0, f1, 0, default);
-            // assume(zero_hashes[..] == reverse(zero_h));
         }
 
-        // method init_zero_hashes(z: array<int>, h: nat, f1 : (int, int) -> int, d: int)
-        //     requires h >= 1
-        //     ensures z[..] == reverse(zeroes(f1, d, h - 1))
-        //     // modifies this.z
-        // {
-        //     // z := new int[h];
-        //     var i := 0 ;
-        //     z[0] := d;
-        //     while i < h - 1 {
-        //         z[i + 1] := f1(z[i], z[i]);
-        //         i := i + 1;
-        //     }
-        //     assume(z[..] == reverse(zeroes(f1, d, h - 1)));
-        // }
-        // for (uint height = 0; height < DEPOSIT_CONTRACT_TREE_DEPTH - 1; height++)
-        //     zero_hashes[height + 1] = sha256(abi.encodePacked(zero_hashes[height], zero_hashes[height]));
-
-
         ///////////////////////////////////////////////////////////////////////////
-        //  Imperative versions of algorithms.
+        //  Imperative versions of algorithms with dynamic array allocations.
         ///////////////////////////////////////////////////////////////////////////
 
+        /**
+         *  This method initialises the array zero_hashes.
+         *  The autocintracts proof implies:
+         *  1. whenever init_zero_hashes() is called, Valid() holds
+         *  2. it follows that it holds if the initilisation happens right after
+         *      the constructor or at any other time later.
+         */
+        method init_zero_hashes()
+            modifies this.zero_hashes
+        {
+            assert(zero_hashes.Length >= 1);
+            var i := 0 ;
+            zero_hashes[0] := d;
+            while i < zero_hashes.Length - 1 
+                invariant 0 <= i <=  zero_hashes.Length - 1
+                invariant zero_hashes[..i + 1] == reverse(zero_h)[..i + 1]
+
+                decreases zero_hashes.Length - i
+            {
+                zero_hashes[i + 1] := f(zero_hashes[i], zero_hashes[i]);
+                i := i + 1;
+            }
+
+            //  Invariant for i == zero_hashes.Length - 1
+            assert(zero_hashes[..] == reverse(zero_h));
+
+        }
+
+       
         /** 
          *  This method updates the left siblings (rBranch) in order
          *  to maintain the correspondence with the Merkle tree for values.
          *  This is captured by the Valid() predicate.
          *  
          *  @param  v   The new deposit amount.
+         *
+         *  @note       The autocontracts attribute impliictely adds the pre and 
+         *              post condition Valid() to the spec of each method.
+         *  
          */
          method {:timeLimitMultiplier 10} deposit(v : int) 
-            // requires Valid()
-            requires count < power2(TREE_HEIGHT) - 1         
-            // ensures Valid()
-            // ensures values == old(values) + [v]
-            // ensures count == old(count) + 1
-            // ensures zero_hashes[..] == old(zero_hashes)[..]
-            // ensures areSiblingsAtIndex(|values|, buildMerkle(values, TREE_HEIGHT, f, d), rBranch, zero_h)
-
+            /** The tree cannot be full.  */
+            requires count < power2(TREE_HEIGHT) - 1     
+            /** The new value `v` should be added to history of received values. */
+            ensures values == old(values) + [v]    
+            
             modifies this, this.branch
         {
             var value := v;
             var size : nat := count;
             var i : nat := 0;
             
+            //  Store the expected result in e.
             ghost var e := computeLeftSiblingsOnNextpathWithIndex(TREE_HEIGHT, old(size), old(rBranch), zero_h, f, v);
-            ghost var p := natToBitList(|values|, TREE_HEIGHT);
            
-            //  In our version rBranch and zero_h store the vectors in reverse order, so we
-            //  use TREE_HEIGHT - i - 1  instead of index i < TREE_HEIGHT in the original algorithm.
-            //  @todo   Add a copy of rBranch in reverse order to use index i.
-            //  Note that the test i < TREE_HEIGHT in the original
-            //  version of the algorithm always evaluates to true and is redundant.
+            //  rBranch and zero_h correspond to  the vectors branch and zero_hashes in reverse
+            //   order, so the index TREE_HEIGHT - i - 1  is used in place if i to dereference them.
             while size % 2 == 1 
-
-                // invariant rBranch == old(rBranch) 
-                // invariant zero_h == old(zero_h) 
-                // invariant branch == old(branch)
-                // invariant zero_hashes == old(zero_hashes)
-                // invariant branch[..] == old(branch[..]) 
-                // invariant zero_hashes[..] == old(zero_hashes[..])
-                // invariant zero_hashes[..] == reverse(zero_h) 
-                // invariant branch[..] == reverse(rBranch)
 
                 invariant 0 <= TREE_HEIGHT - i - 1 < |rBranch| == branch.Length
                 invariant 0 <= size < power2(TREE_HEIGHT - i) - 1
                 
-                // invariant branch.Length == |rBranch| == |e| == |zero_h| == TREE_HEIGHT
-
                 //  Main invariant:
                 invariant e == 
                     computeLeftSiblingsOnNextpathWithIndex(
@@ -230,13 +228,11 @@ module DepositSmart {
                 //  Termination is easy as size decreases and must be zero.
                 decreases size 
             {
-
-                ghost var i' := TREE_HEIGHT - i;
-                // ghost var v' := value;
-                // ghost var s' := size / 2; 
+                //  This is not an invarint but true if siez % 2 == 1 and 
+                //  pre-condition for mainInvariantProofHelper
                 assert(0 != size);
 
-
+                //  The proof steps for the main invariant,
                 calc == {
                     e;
                     computeLeftSiblingsOnNextpathWithIndex(
@@ -244,15 +240,6 @@ module DepositSmart {
                         take(rBranch, TREE_HEIGHT - i), 
                         take(zero_h, TREE_HEIGHT - i), f, value) 
                     + drop(rBranch, TREE_HEIGHT - i);
-                    // calc == {
-                    //     TREE_HEIGHT - i;
-                    //     i';
-                    // }
-                    // computeLeftSiblingsOnNextpathWithIndex(
-                    //     i', size, 
-                    //     take(rBranch, i'), 
-                    //     take(zero_h, i'), f, value) 
-                    // + drop(rBranch, i');
                     { mainInvariantProofHelper(TREE_HEIGHT - i, size, rBranch, zero_h, f, value); }
                     computeLeftSiblingsOnNextpathWithIndex(
                         TREE_HEIGHT - i - 1, size / 2, 
@@ -260,16 +247,12 @@ module DepositSmart {
                         take(zero_h, TREE_HEIGHT - i - 1), f,  f(rBranch[TREE_HEIGHT - i - 1], value)) 
                     + drop(rBranch, TREE_HEIGHT - i - 1);
                 }
-                // assert(rBranch[TREE_HEIGHT - i - 1] == branch[i]);
+
+                // Algorithm
                 value := f(branch[i], value);
                 size := size / 2;
                 i := i + 1;
-
-                // mainInvariantProofHelper(TREE_HEIGHT -old(i), old(size), rBranch, zero_h, f, old(value));
-                // assert(s' == size);
-                // assert(i' - 1 == TREE_HEIGHT - i);
-                // assert(value == f(rBranch[i' - 1], v'));
-                
+    
             }
             //  Show that e == rBranch[TREE_HEIGHT - i - 1 := value]
             calc == {
@@ -292,40 +275,30 @@ module DepositSmart {
                 rBranch[TREE_HEIGHT - i - 1 := value];
                 old(rBranch)[TREE_HEIGHT - i - 1 := value];
             }
-            //  This is the important hidden property: TREE_HEIGHT - i - 1 ( i < TREE_HEIGHT)
-            //  in original version) is NEVER out of range, and always in [0, TREE_HEIGHT[
+            //  This is the important hidden property: 0 <= TREE_HEIGHT - i - 1 < |rBranch|
+            //  and also 0 <= i < brancvh.Lenhth 
+            //  This proves that in the original version, i is NEVER out of range, 
+            //  and always in [0, branch.Lenhth[
             rBranch := rBranch[TREE_HEIGHT - i - 1 := value];
 
-            //  if follows that 0 <= i < |branch|
-            // branch := branch[i := value];
+            //  if follows that 0 <= i < |branch| and no index-out-of-bounds
             branch[i] := value;
 
+            //  Some hints for the proof of the post conditions.
             assert(rBranch == old(rBranch)[TREE_HEIGHT - i - 1 := value] == e);
             assert(branch[..] == old(branch)[..][i := value]);
             assert(branch[..] == reverse(rBranch));
+
             //  Finally increment count. Note that count can be incremented at the beginning
             //  provided that the while loop condition is flipped to sizeA % 2 == 0.
             count := count + 1;
-            //  Update values
+
+            //  Update (ghost) values
             values := values + [v];
            
-        //    assert(areSiblingsAtIndex(|old(values)|, buildMerkle(old(values), TREE_HEIGHT, f, d), old(rBranch), zero_h));
-            //  Use correctness lemma  
-        // assert(zero_hashes[..] == old(zero_hashes)[..]);
-        // assert(zero_h == old(zero_h) == zeroes(f, d, TREE_HEIGHT - 1));
-        // assert(values == old(values) + [v]);
-        assert(count == old(count) + 1 == |values| == |old(values)| + 1);
-        computeNewLeftIsCorrect(old(values), v, TREE_HEIGHT, old(rBranch), zero_h, f, d);
-        assert(areSiblingsAtIndex(|values|, buildMerkle(values, TREE_HEIGHT, f, d), rBranch, zero_h));
-        // assume(zero_h == zeroes(f, d, TREE_HEIGHT - 1));
-        // assume(1 <= TREE_HEIGHT == branch.Length == |rBranch| == |zero_h|);
-        // assume(branch[..] == reverse(rBranch));
-            //  Maximum number of values stored in the tree bounded.
-        // assume(count < power2(TREE_HEIGHT)); 
-            //  count is the number of values added so far and should correspond to |values|.
-        // assume(|values| == count);
-            //  zero_h is constant and equal to default values for each level of t.
-        // assume(zero_hashes[..] == old(zero_hashes[..]));
+            assert(count == old(count) + 1 == |values| == |old(values)| + 1);
+            computeNewLeftIsCorrect(old(values), v, TREE_HEIGHT, old(rBranch), zero_h, f, d);
+            assert(areSiblingsAtIndex(|values|, buildMerkle(values, TREE_HEIGHT, f, d), rBranch, zero_h));
         }
 
         /**
@@ -395,21 +368,14 @@ module DepositSmart {
          *  This method should always return the root value of the tree.
          *
          *  @returns    The root value of the Merkle Tree for values.
+         *
+         *  @note       The autocontracts attribute impliictely adds the pre and 
+         *              post condition Valid() to the spec of each method.
          */
          method {:timeLimitMultiplier 8} get_deposit_root() returns (r : int) 
-            // requires Valid()
-            // requires branch == reverse(rBranch)
-            // ensures Valid()
-            // ensures branch == reverse(rBranch)
             /** The result of get_deposit_root_() is the root value of the Merkle tree for values.  */
             ensures r == buildMerkle(values, TREE_HEIGHT, f, d).v 
-            modifies {}
-            // reads {this, this.branch}
         {
-            //  Some help to prove that the main invariant holds on entry:
-            assert(take(rBranch, TREE_HEIGHT) == rBranch);
-            assert(take(zero_h, TREE_HEIGHT) == zero_h);
-
             //  Store the expected result in a ghost variable.
             ghost var e := computeRootLeftRightUpWithIndex(TREE_HEIGHT, count, rBranch, zero_h, f, d);
 
@@ -431,12 +397,13 @@ module DepositSmart {
 
                 decreases TREE_HEIGHT - h 
             {
-                //  A little help for Dafny to check the proof:
+                //  A little help for Dafny to check the proof of the main invariant
                 assert(last(take(rBranch, TREE_HEIGHT - h)) == rBranch[TREE_HEIGHT - h - 1]);
                 assert(last(take(zero_h, TREE_HEIGHT - h)) == zero_h[TREE_HEIGHT - h - 1]);
                 assert(init(take(rBranch, TREE_HEIGHT - h)) == take(rBranch, TREE_HEIGHT - h - 1));
                 assert(init(take(zero_h, TREE_HEIGHT - h)) == take(zero_h, TREE_HEIGHT - h - 1));
 
+                //  Algorithm 
                 if size % 2 == 1 {
                     assert(rBranch[TREE_HEIGHT - h - 1] == branch[h]);
                     r := f(branch[h], r);
